memcpy.v
@@ -1,3 +1,4 @@
+From iris.base_logic.lib Require Import namespaces.
 From lrust Require Export notation.
 From lrust Require Import heap proofmode.
 
